src/HOL/BNF/BNF_GFP.thy
@@ -276,23 +276,14 @@ lemma fromCard_toCard:
 unfolding fromCard_def by (rule some_equality) (auto simp add: toCard_inj)
 
 (* pick according to the weak pullback *)
-definition pickWP_pred where
-"pickWP_pred A p1 p2 b1 b2 a \<equiv> a \<in> A \<and> p1 a = b1 \<and> p2 a = b2"
-
 definition pickWP where
-"pickWP A p1 p2 b1 b2 \<equiv> SOME a. pickWP_pred A p1 p2 b1 b2 a"
+"pickWP A p1 p2 b1 b2 \<equiv> SOME a. a \<in> A \<and> p1 a = b1 \<and> p2 a = b2"
 
 lemma pickWP_pred:
 assumes "wpull A B1 B2 f1 f2 p1 p2" and
 "b1 \<in> B1" and "b2 \<in> B2" and "f1 b1 = f2 b2"
-shows "\<exists> a. pickWP_pred A p1 p2 b1 b2 a"
-using assms unfolding wpull_def pickWP_pred_def by blast
-
-lemma pickWP_pred_pickWP:
-assumes "wpull A B1 B2 f1 f2 p1 p2" and
-"b1 \<in> B1" and "b2 \<in> B2" and "f1 b1 = f2 b2"
-shows "pickWP_pred A p1 p2 b1 b2 (pickWP A p1 p2 b1 b2)"
-unfolding pickWP_def using assms by(rule someI_ex[OF pickWP_pred])
+shows "\<exists> a. a \<in> A \<and> p1 a = b1 \<and> p2 a = b2"
+using assms unfolding wpull_def by blast
 
 lemma pickWP:
 assumes "wpull A B1 B2 f1 f2 p1 p2" and
@@ -300,7 +291,7 @@ assumes "wpull A B1 B2 f1 f2 p1 p2" and
 shows "pickWP A p1 p2 b1 b2 \<in> A"
       "p1 (pickWP A p1 p2 b1 b2) = b1"
       "p2 (pickWP A p1 p2 b1 b2) = b2"
-using assms pickWP_pred_pickWP unfolding pickWP_pred_def by fastforce+
+unfolding pickWP_def using assms someI_ex[OF pickWP_pred] by fastforce+
 
 lemma Inl_Field_csum: "a \<in> Field r \<Longrightarrow> Inl a \<in> Field (r +c s)"
 unfolding Field_card_of csum_def by auto
